\documentclass{article}
\usepackage{amsmath}
\usepackage{amsthm}
\usepackage{array}

% Define a new theorem environment
\newtheorem*{thm}{Theorem}
% Make a centering column type of a given width.
\newcolumntype{C}[1]{>{\hfil}p{#1}<{\hfil}}

\title{Example proof}
\author{Stephen Checkoway}

\begin{document}
\maketitle

We want to prove the following theorem.
\begin{thm}
Let $\Sigma$ be a finite alphabet and let $w\in\Sigma^*$ be a word of
length at least~2. If there exist nonempty words $x,y\in\Sigma^+$
such that $w=xy=yx$, then there exists a nonempty word $z\in\Sigma^+$
and positive integers $a$ and~$b$ such that $x=z^a$ and $y=z^b$.
\end{thm}

\begin{proof}
We will prove the theorem by induction on the length of $w$. The base
case is $|w|=2$. This case is trivial since it must be the case that
$|x|=|y|=1$. Therefore, $x=y$ so $z=x$ and $a=b=1$.

For the inductive step, assume that the theorem holds for all words of
length less than~$m$. Let $w$ be a word of length~$m$ such that
$w=xy=yx$ for nonempty $x$ and~$y$. Write $x=x_1 x_2 \cdots x_k$ and
$y=y_1 y_2 \cdots y_n$. We can assume, without loss of generality,
that $k\le n$ (otherwise swap $x$ and~$y$).

If $k=n$, then since $xy=yx$, we have $x_1=y_1$, $x_2=y_2$, \ldots,
$x_k=y_k$. Therefore, $x=y$ and we can set $z=x$ and $a=b=1$.

Otherwise, $k<n$ and we have a situation that looks like this.

\begin{center}
\begin{tabular}{|C{2cm}|C{3cm}|}
\hline
$x$ & $y$\\
\hline
\end{tabular}

\vspace{.5\baselineskip}

\begin{tabular}{|C{3cm}|C{2cm}|}
\hline
$y$ & $x$\\
\hline
\end{tabular}
\end{center}

From the picture, it's clear that $y$ starts with $x$ and ends
with the first $n-k$ letters in $y$. Formally, $y=xy_1y_2\cdots
y_{n-k}$. Similarly, $y$ ends with $x$ so $y=y_1y_2\cdots y_{n-k}x$.
Define $y'=y_1y_2\cdots y_{n-k}$. Thus,
\[ y=xy'=y'x \]
and we can apply the inductive hypothesis since $|y|=n<|w|=m$. In
particular, there is a word $z$ and integers $a,c$ such that $x=z^a$
and $y'=z^c$. This gives
\begin{align*}
x&=z^a,\\
y&=xy'=z^az^c=z^{a+c}.
\end{align*}
Setting $b=a+c$ proves the theorem.
\end{proof}

\end{document}
